HOL-Light/x86: Add correctness proof for decompress_d4
Signed-off-by: Hanno Becker <beckphan@amazon.co.uk>

proofs/hol_light/x86_64/proofs/mlkem_poly_decompress_d4.ml
@@ -230,4 +230,212 @@ let mlkem_poly_decompress_d4_mc =
 ];;
 (*** BYTECODE END ***)
 
-(* TODO: Prove correctness of poly_decompress_d4_avx2 *)
+let mlkem_poly_decompress_d4_tmc =
+  define_trimmed "mlkem_poly_decompress_d4_tmc" mlkem_poly_decompress_d4_mc;;
+let MLKEM_POLY_DECOMPRESS_D4_TMC_EXEC =
+  X86_MK_CORE_EXEC_RULE mlkem_poly_decompress_d4_tmc;;
+
+(* ------------------------------------------------------------------------- *)
+(* Code length constants                                                     *)
+(* ------------------------------------------------------------------------- *)
+
+let LENGTH_MLKEM_POLY_DECOMPRESS_D4_MC =
+  REWRITE_CONV[mlkem_poly_decompress_d4_mc] `LENGTH mlkem_poly_decompress_d4_mc`
+  |> CONV_RULE (RAND_CONV LENGTH_CONV);;
+
+let LENGTH_MLKEM_POLY_DECOMPRESS_D4_TMC =
+  REWRITE_CONV[mlkem_poly_decompress_d4_tmc] `LENGTH mlkem_poly_decompress_d4_tmc`
+  |> CONV_RULE (RAND_CONV LENGTH_CONV);;
+
+let LENGTH_SIMPLIFY_CONV =
+  REWRITE_CONV[LENGTH_MLKEM_POLY_DECOMPRESS_D4_MC;
+               LENGTH_MLKEM_POLY_DECOMPRESS_D4_TMC] THENC
+  NUM_REDUCE_CONV THENC REWRITE_CONV[ADD_0];;
+
+(* ------------------------------------------------------------------------- *)
+(* Word-expression for decompression computed by the AVX2 assembly           *)
+(* ------------------------------------------------------------------------- *)
+
+let decompress_d4_avx2 = new_definition `decompress_d4_avx2 (x : 4 word) : 16 word =
+   word_subword (word_add (word_ushr
+     (word_mul (word_sx (word_mul (word_zx x : 16 word) (word 2048 : 16 word)) : 32 word) (word 3329 : 32 word))
+     14) (word 1)) (1, 16)`;;
+
+let DECOMPRESS_D4_AVX2_CORRECT = prove(
+  `decompress_d4_avx2 x = decompress_d4 x`,
+  let DIMINDEX_4 = DIMINDEX_CONV `dimindex(:4)` in
+  let VAL_4_WORD_BOUND = WORD_BLAST `val (x : 4 word) < 16` in
+  let VAL_16_WORD_BOUND = WORD_BLAST `val (x : 16 word) < 65536` in
+  let VAL_DECOMPRESS_D4_AVX2_CORE = prove(`!(x: 16 word).
+    val (word_subword
+          (word_add
+             (word_ushr
+                (word_shl (word_zx x : 32 word) 11)
+                14)
+             (word 1))
+           (1,16) : 16 word)
+      = (val x + 8) DIV 16`,
+    GEN_TAC THEN
+    REWRITE_TAC [WORD_BLAST `!(x : 16 word). word_ushr (word_shl (word_zx x : 32 word) 11) 14 = word_ushr (word_zx x) 3`] THEN
+    REWRITE_TAC[VAL_WORD_SUBWORD; VAL_WORD_ADD; VAL_WORD_USHR; VAL_WORD_SHL;
+                VAL_WORD_ZX_GEN; VAL_WORD; DIMINDEX_16; DIMINDEX_32] THEN
+    CONV_TAC NUM_REDUCE_CONV THEN MP_TAC VAL_16_WORD_BOUND THEN STRIP_TAC THEN
+    MAP_EVERY (fun t -> SUBGOAL_THEN t SUBST1_TAC THENL [MATCH_MP_TAC MOD_LT THEN ASM_ARITH_TAC; ALL_TAC])
+      [`val (x:16 word) MOD 4294967296 = val x`;
+       `(val (x:16 word) DIV 8 + 1) MOD 4294967296 = val x DIV 8 + 1`;
+       `((val (x:16 word) DIV 8 + 1) DIV 2) MOD 65536 = (val x DIV 8 + 1) DIV 2`] THEN
+    ASM_ARITH_TAC) in
+  let VAL_DECOMPRESS_D4 = prove(
+    `val (decompress_d4 x) = (val x * 3329 + 8) DIV 16`,
+    IMP_REWRITE_TAC [decompress_d4; VAL_WORD_EQ; DIMINDEX_16] THEN MP_TAC VAL_4_WORD_BOUND THEN ARITH_TAC) in
+  let MUL_ZX_SHUFFLE = prove(`!(x : 4 word). word_mul (word 3329) (word_zx x : 32 word) = word_zx (word_mul (word 3329) (word_zx x : 16 word))`,
+    GEN_TAC THEN
+    REWRITE_TAC[GSYM VAL_EQ; VAL_WORD_MUL; VAL_WORD_ZX_GEN; VAL_WORD;
+                DIMINDEX_4; DIMINDEX_16; DIMINDEX_32] THEN
+    CONV_TAC NUM_REDUCE_CONV THEN
+    MP_TAC VAL_4_WORD_BOUND THEN STRIP_TAC THEN
+    CONV_TAC MOD_DOWN_CONV THEN
+    AP_THM_TAC THEN AP_TERM_TAC THEN
+    MATCH_MP_TAC(GSYM MOD_LT) THEN ASM_ARITH_TAC) in
+  let TECHNICAL_EQ = prove(
+    `word_sx (word_mul (word_zx (x:4 word):16 word) (word 2048:16 word)):32 word
+     = word_shl (word_zx (x:4 word):32 word) 11`,
+     REWRITE_TAC [WORD_BLAST `!(x : 16 word). word_mul x (word 2048 : 16 word) = word_shl x 11`] THEN CONV_TAC WORD_BLAST) in
+  REWRITE_TAC [GSYM VAL_EQ;decompress_d4_avx2; MUL_ZX_SHUFFLE; VAL_DECOMPRESS_D4; VAL_DECOMPRESS_D4_AVX2_CORE; TECHNICAL_EQ; WORD_MUL_SHL] THEN
+  IMP_REWRITE_TAC [VAL_WORD_MUL_EXACT; VAL_WORD_EXACT; VAL_WORD_ZX_EXACT; DIMINDEX_4; DIMINDEX_16] THEN
+  NUM_REDUCE_TAC THEN MP_TAC VAL_4_WORD_BOUND THEN ARITH_TAC);;
+
+(* ------------------------------------------------------------------------- *)
+(* Main correctness theorem                                                  *)
+(* ------------------------------------------------------------------------- *)
+
+let WORD_AND_8_4_4_15 = prove(
+   `word_and (word_join (x:8 word) (word_join (b:4 word) (a:4 word):8 word))
+             (word 15:16 word) = word_zx a`, CONV_TAC WORD_BLAST);;
+let WORD_AND_8_4_4_240 = prove(
+   `word_and (word_join (x:8 word) (word_join (b:4 word) (a:4 word):8 word))
+             (word 240:16 word) = word_shl (word_zx b) 4`, CONV_TAC WORD_BLAST);;
+let WORD_SHL_THEN_MUL_2048 = prove(
+      `(word_mul (word_shl (word_zx (x : 4 word) : 16 word) 4) (word 128)) = word_mul (word_zx x : 16 word) (word 2048)`,
+      CONV_TAC WORD_BLAST);;
+
+let MLKEM_POLY_DECOMPRESS_D4_CORRECT = prove(
+  `!r a data (inlist:(4 word) list) pc.
+      LENGTH inlist = 256 /\
+      aligned 32 r /\
+      aligned 32 data /\
+      ALL (nonoverlapping (r, 512))
+          [(word pc, LENGTH mlkem_poly_decompress_d4_tmc); (a, 128); (data, 32)]
+      ==> ensures x86
+           (\s. bytes_loaded s (word pc) (BUTLAST mlkem_poly_decompress_d4_tmc) /\
+                read RIP s = word pc /\
+                C_ARGUMENTS [r; a; data] s /\
+                read (memory :> bytes(data, 32)) s =
+                  num_of_wordlist ((MAP iword decompress_d4_data): (8 word) list) /\
+                read (memory :> bytes(a, 128)) s = num_of_wordlist inlist)
+           (\s. read RIP s = word (pc + 624) /\
+                read (memory :> bytes(r, 512)) s = num_of_wordlist (MAP decompress_d4 inlist))
+           (MAYCHANGE [events] ,,
+            MAYCHANGE [memory :> bytes(r, 512)] ,,
+            MAYCHANGE [RIP] ,, MAYCHANGE [RAX] ,,
+            MAYCHANGE [ZMM0; ZMM1; ZMM2; ZMM3; ZMM4])`,
+  MAP_EVERY X_GEN_TAC
+    [`r:int64`; `a:int64`; `data:int64`; `inlist:(4 word) list`; `pc:num`] THEN
+  CONV_TAC LENGTH_SIMPLIFY_CONV THEN
+  REWRITE_TAC[MAYCHANGE_REGS_AND_FLAGS_PERMITTED_BY_ABI; C_ARGUMENTS;
+              NONOVERLAPPING_CLAUSES; ALL] THEN
+  DISCH_THEN(REPEAT_TCL CONJUNCTS_THEN ASSUME_TAC) THEN
+  (* Move to 256-bit granular preconditions for input array *)
+  ENSURES_INIT_TAC "s0" THEN
+  UNDISCH_TAC `read(memory :> bytes(a,128)) s0 = num_of_wordlist(inlist: (4 word) list)` THEN
+  GEN_REWRITE_TAC (LAND_CONV o RAND_CONV o RAND_CONV) [GSYM LIST_OF_SEQ_EQ_SELF] THEN
+  ASM_REWRITE_TAC[] THEN
+  CONV_TAC(LAND_CONV(RAND_CONV(RAND_CONV LIST_OF_SEQ_CONV))) THEN
+  REWRITE_TAC[] THEN
+  REPLICATE_TAC 4 (GEN_REWRITE_TAC (LAND_CONV o ONCE_DEPTH_CONV)
+                   [GSYM NUM_OF_PAIR_WORDLIST]) THEN
+  REWRITE_TAC[pair_wordlist] THEN CONV_TAC WORD_REDUCE_CONV THEN
+  CONV_TAC(LAND_CONV BYTES_EQ_NUM_OF_WORDLIST_EXPAND_CONV) THEN
+  REWRITE_TAC[GSYM BYTES64_WBYTES] THEN STRIP_TAC THEN
+  (* Move to 256-bit granular precondition for constant array *)
+  UNDISCH_TAC
+   `read(memory :> bytes(data,32)) s0 = num_of_wordlist ((MAP iword decompress_d4_data) : (8 word) list)` THEN
+  REWRITE_TAC [decompress_d4_data; MAP] THEN
+  REPLICATE_TAC 5 (GEN_REWRITE_TAC (LAND_CONV o ONCE_DEPTH_CONV)
+                   [GSYM NUM_OF_PAIR_WORDLIST]) THEN
+  REWRITE_TAC[pair_wordlist] THEN CONV_TAC WORD_REDUCE_CONV THEN
+  CONV_TAC(LAND_CONV BYTES_EQ_NUM_OF_WORDLIST_EXPAND_CONV) THEN
+  REWRITE_TAC[GSYM BYTES256_WBYTES] THEN STRIP_TAC THEN
+  (*** Symbolic execution ***)
+  MAP_EVERY (fun n -> X86_STEPS_TAC MLKEM_POLY_DECOMPRESS_D4_TMC_EXEC [n] THEN
+                      SIMD_SIMPLIFY_TAC [GSYM WORD_AND_8_4_4_15; GSYM WORD_AND_8_4_4_240; GSYM WORD_SHL_THEN_MUL_2048; decompress_d4_avx2; GSYM DECOMPRESS_D4_AVX2_CORRECT])
+            (1--122) THEN
+  ENSURES_FINAL_STATE_TAC THEN ASM_REWRITE_TAC[] THEN
+  (* Spell out input list entry by entry *)
+  GEN_REWRITE_TAC (RAND_CONV o RAND_CONV o RAND_CONV) [GSYM LIST_OF_SEQ_EQ_SELF] THEN
+  ASM_REWRITE_TAC[LENGTH_MAP] THEN
+  CONV_TAC (TOP_SWEEP_CONV LIST_OF_SEQ_CONV) THEN
+  REWRITE_TAC [MAP] THEN
+  (* Switch to 256-bit granularity *)
+  REPLICATE_TAC 4 (CONV_TAC (ONCE_REWRITE_CONV [GSYM NUM_OF_PAIR_WORDLIST])) THEN
+  REWRITE_TAC[pair_wordlist] THEN
+  CONV_TAC (ONCE_DEPTH_CONV BYTES_EQ_NUM_OF_WORDLIST_EXPAND_CONV) THEN
+  ASM_REWRITE_TAC[GSYM BYTES256_WBYTES]);;
+
+let MLKEM_POLY_DECOMPRESS_D4_NOIBT_SUBROUTINE_CORRECT = prove(
+  `!r a data (inlist:(4 word) list) pc stackpointer returnaddress.
+      LENGTH inlist = 256 /\
+      aligned 32 r /\
+      aligned 32 data /\
+      ALL (nonoverlapping (r, 512))
+          [(word pc, LENGTH mlkem_poly_decompress_d4_tmc); (a, 128); (data, 32); (stackpointer, 8)]
+      ==> ensures x86
+           (\s. bytes_loaded s (word pc) mlkem_poly_decompress_d4_tmc /\
+                read RIP s = word pc /\
+                read RSP s = stackpointer /\
+                read (memory :> bytes64 stackpointer) s = returnaddress /\
+                C_ARGUMENTS [r; a; data] s /\
+                read (memory :> bytes(data, 32)) s =
+                  num_of_wordlist ((MAP iword decompress_d4_data): (8 word) list) /\
+                read (memory :> bytes(a, 128)) s = num_of_wordlist inlist)
+           (\s. read RIP s = returnaddress /\
+                read RSP s = word_add stackpointer (word 8) /\
+                read (memory :> bytes(r, 512)) s = num_of_wordlist (MAP decompress_d4 inlist) /\
+                (!i. i < 256 ==> &0 <= ival (EL i (MAP decompress_d4 inlist)) /\
+                                       ival (EL i (MAP decompress_d4 inlist)) < &3329))
+           (MAYCHANGE [RSP] ,,
+            MAYCHANGE_REGS_AND_FLAGS_PERMITTED_BY_ABI ,,
+            MAYCHANGE [memory :> bytes(r, 512)])`,
+  X86_PROMOTE_RETURN_NOSTACK_TAC mlkem_poly_decompress_d4_tmc
+    MLKEM_POLY_DECOMPRESS_D4_CORRECT THEN
+  (* Prove bounds *)
+  REPEAT STRIP_TAC THEN ASM_SIMP_TAC [EL_MAP; ARITH; IVAL_DECOMPRESS_D4_BOUND]);;
+
+(* NOTE: This must be kept in sync with the CBMC specification
+ * in mlkem/src/native/x86_64/src/arith_native_x86_64.h *)
+
+let MLKEM_POLY_DECOMPRESS_D4_SUBROUTINE_CORRECT = prove(
+  `!r a data (inlist:(4 word) list) pc stackpointer returnaddress.
+      LENGTH inlist = 256 /\
+      aligned 32 r /\
+      aligned 32 data /\
+      ALL (nonoverlapping (r, 512))
+          [(word pc, LENGTH mlkem_poly_decompress_d4_mc); (a, 128); (data, 32); (stackpointer, 8)]
+      ==> ensures x86
+           (\s. bytes_loaded s (word pc) mlkem_poly_decompress_d4_mc /\
+                read RIP s = word pc /\
+                read RSP s = stackpointer /\
+                read (memory :> bytes64 stackpointer) s = returnaddress /\
+                C_ARGUMENTS [r; a; data] s /\
+                read (memory :> bytes(data, 32)) s =
+                  num_of_wordlist ((MAP iword decompress_d4_data): (8 word) list) /\
+                read (memory :> bytes(a, 128)) s = num_of_wordlist inlist)
+           (\s. read RIP s = returnaddress /\
+                read RSP s = word_add stackpointer (word 8) /\
+                read (memory :> bytes(r, 512)) s = num_of_wordlist (MAP decompress_d4 inlist) /\
+                (!i. i < 256 ==> &0 <= ival (EL i (MAP decompress_d4 inlist)) /\
+                                       ival (EL i (MAP decompress_d4 inlist)) < &3329))
+           (MAYCHANGE [RSP] ,,
+            MAYCHANGE_REGS_AND_FLAGS_PERMITTED_BY_ABI ,,
+            MAYCHANGE [memory :> bytes(r, 512)])`,
+  MATCH_ACCEPT_TAC(ADD_IBT_RULE MLKEM_POLY_DECOMPRESS_D4_NOIBT_SUBROUTINE_CORRECT));;
